### State Representation
In SLAM, the state vector $\mathbf{x}$ encapsulates the robot's pose and the map features:
$$\mathbf{x}_t = \begin{bmatrix} \mathbf{x}_{robot} \\ \mathbf{x}_{map} \end{bmatrix}$$

- **Robot Pose**: $\mathbf{x}_{robot}$ typically includes <mark style="background: #FFB8EBA6;">position and orientation</mark>.
- **Map Features**: $\mathbf{x}_{map}$ includes the <mark style="background: #FF5582A6;">coordinates of landmarks or features</mark> in the environment.

### Motion Model
The motion model predicts the <mark style="background: #FFB86CA6;">next state of the robot based on its current state and control inputs</mark>:
$$\mathbf{x}_t = f(\mathbf{x}_{t-1}, \mathbf{u}_t) + \mathbf{w}_t$$
where:
- $\mathbf{x}_{t-1}$ is the previous state.
- $\mathbf{u}_t$ is the control input (e.g., velocity, steering angle).
- $f$ is the nonlinear motion model function.
- $\mathbf{w}_t$ is the process noise, often modeled as zero-mean Gaussian noise: $\mathbf{w}_t \sim \mathcal{N}(0, \mathbf{Q}_t)$.

**Example**:
For a simple 2D robot, the motion model can be:
$$\begin{bmatrix} x_t \\ y_t \\ \theta_t \end{bmatrix} = \begin{bmatrix} x_{t-1} \\ y_{t-1} \\ \theta_{t-1} \end{bmatrix} + \begin{bmatrix} v_t \cos(\theta_{t-1}) \\ v_t \sin(\theta_{t-1}) \\ \omega_t \end{bmatrix} + \mathbf{w}_t$$
where $v_t$ is the linear velocity, $\omega_t$ is the angular velocity.

### Observation Model
The observation model <mark style="background: #FFF3A3A6;">relates the state of the robot and the map to the sensor measurements</mark>:
$$\mathbf{z}_t = h(\mathbf{x}_t) + \mathbf{v}_t$$
where:
- $\mathbf{z}_t$ is the observation (sensor measurement).
- $h$ is the nonlinear observation model function.
- $\mathbf{v}_t$ is the observation noise, often modeled as zero-mean Gaussian noise: $\mathbf{v}_t \sim \mathcal{N}(0, \mathbf{R}_t)$.

**Example**:
For a range-bearing sensor, the observation model might be:
$$\mathbf{z}_t = \begin{bmatrix} r \\ \phi \end{bmatrix} = \begin{bmatrix} \sqrt{(x - x_L)^2 + (y - y_L)^2} \\ \arctan\left(\frac{y - y_L}{x - x_L}\right) - \theta \end{bmatrix} + \mathbf{v}_t$$
where $(x_L, y_L)$ are the <mark style="background: #BBFABBA6;">coordinates of a landmark</mark>, $r$ is the range, and $\phi$ is the bearing.

### Bayesian Filtering
SLAM often uses Bayesian filtering to estimate the state distribution over time.

#### Prediction Step
The prediction step uses the motion model to estimate the state and covariance:
$$\mathbf{\hat{x}}_t^- = f(\mathbf{\hat{x}}_{t-1}, \mathbf{u}_t)$$
$$\mathbf{P}_t^- = \mathbf{F}_t \mathbf{P}_{t-1} \mathbf{F}_t^T + \mathbf{Q}_t$$
where:
-  $\mathbf{\hat{x}}_t^-$ is the predicted state.
- $\mathbf{P}_t^-$ is the predicted covariance.
- $\mathbf{F}_t$ is the Jacobian of $f$ with respect to $\mathbf{x}$.

**Example**:
For a linear motion model:
$$f(\mathbf{x}, \mathbf{u}) = \mathbf{A} \mathbf{x} + \mathbf{B} \mathbf{u}$$
$$\mathbf{F}_t = \mathbf{A}$$

#### Update Step
The update step incorporates the observation model to correct the predicted state:
$$\mathbf{y}_t = \mathbf{z}_t - h(\mathbf{\hat{x}}_t^-) $$
$$\mathbf{S}_t = \mathbf{H}_t \mathbf{P}_t^- \mathbf{H}_t^T + \mathbf{R}_t$$
$$\mathbf{K}_t = \mathbf{P}_t^- \mathbf{H}_t^T \mathbf{S}_t^{-1}$$
$$\mathbf{\hat{x}}_t = \mathbf{\hat{x}}_t^- + \mathbf{K}_t \mathbf{y}_t$$
$$\mathbf{P}_t = (\mathbf{I} - \mathbf{K}_t \mathbf{H}_t) \mathbf{P}_t^-$$
where:
- $\mathbf{y}_t$ is the innovation.
- $\mathbf{S}_t$ is the innovation covariance.
- $\mathbf{K}_t$ is the Kalman gain.
- $\mathbf{H}_t$ is the Jacobian of $h$ with respect to $\mathbf{x}$.

**Example**:
For a linear observation model:
$$h(\mathbf{x}) = \mathbf{C} \mathbf{x}$$
$$\mathbf{H}_t = \mathbf{C}$$

### Graph-Based SLAM
Graph-based SLAM represents the problem as a graph optimization problem, minimizing the error in the constraints.

#### Graph Representation
- **Nodes**: Represent <mark style="background: #FFB8EBA6;">robot poses and landmarks</mark>.
- **Edges**: Represent <mark style="background: #ABF7F7A6;">constraints (measurements)</mark> between nodes.

#### Optimization Problem
The optimization problem is to find the state $\mathbf{x}$ that minimizes the overall error:
$$\min_{\mathbf{x}} \sum_{i,j} \| \mathbf{z}_{ij} - h(\mathbf{x}_i, \mathbf{x}_j) \|^2_{\mathbf{\Omega}_{ij}}$$
where:
- $\mathbf{z}_{ij}$ is the measurement between nodes $i$ and $j$.
- $h(\mathbf{x}_i, \mathbf{x}_j)$ is the expected measurement.
- $\mathbf{\Omega}_{ij}$ is the information matrix of the measurement.

**Example**:
For a 2D pose graph, the error term for an edge between nodes $i$ and $j$ could be:
$$\mathbf{e}_{ij} = \mathbf{z}_{ij} - \begin{bmatrix} \sqrt{(x_i - x_j)^2 + (y_i - y_j)^2} \\ \arctan\left(\frac{y_i - y_j}{x_i - x_j}\right) - (\theta_i - \theta_j) \end{bmatrix}$$

---

### Detailed Example: SLAM Update Step with Matrix Calculation

We'll use the following assumptions:
1. The robot's state vector consists of position (x, y) and orientation (Î¸).
2. Linear motion model: $$f(\mathbf{x}, \mathbf{u}) = \mathbf{A} \mathbf{x} + \mathbf{B} \mathbf{u}$$
3. Linear observation model: $$h(\mathbf{x}) = \mathbf{C} \mathbf{x}$$
4. The initial state and covariance are given.
5. The control input and observation are given.
6. Process noise $\mathbf{Q}_t$ and observation noise $\mathbf{R}_t$ are given.

#### Initial State and Covariance

$$\mathbf{\hat{x}}_{t-1} = \begin{bmatrix} 2 \\ 3 \\ 0.1 \end{bmatrix}, \quad \mathbf{P}_{t-1} = \begin{bmatrix} 0.1 & 0 & 0 \\ 0 & 0.1 & 0 \\ 0 & 0 & 0.1 \end{bmatrix}$$

#### Control Input

$$\mathbf{u}_t = \begin{bmatrix} 1 \\ 0.1 \end{bmatrix} \quad \text{(linear velocity, angular velocity)}$$

#### Process Noise Covariance

$$\mathbf{Q}_t = \begin{bmatrix} 0.01 & 0 & 0 \\ 0 & 0.01 & 0 \\ 0 & 0 & 0.01 \end{bmatrix}$$

#### Observation

$$\mathbf{z}_t = \begin{bmatrix} 2.1 \\ 3.1 \end{bmatrix} \quad \text{(observed position)}$$

#### Observation Noise Covariance

$$\mathbf{R}_t = \begin{bmatrix} 0.05 & 0 \\ 0 & 0.05 \end{bmatrix}$$

### Step-by-Step Calculation

1. **Prediction Step**

   $$\mathbf{A} = \begin{bmatrix} 1 & 0 & 0 \\ 0 & 1 & 0 \\ 0 & 0 & 1 \end{bmatrix}, \quad \mathbf{B} = \begin{bmatrix} \cos(0.1) & 0 \\ \sin(0.1) & 0 \\ 0 & 1 \end{bmatrix}$$

   $$\mathbf{\hat{x}}_t^- = \mathbf{A} \mathbf{\hat{x}}_{t-1} + \mathbf{B} \mathbf{u}_t = \begin{bmatrix} 1 & 0 & 0 \\ 0 & 1 & 0 \\ 0 & 0 & 1 \end{bmatrix} \begin{bmatrix} 2 \\ 3 \\ 0.1 \end{bmatrix} + \begin{bmatrix} \cos(0.1) & 0 \\ \sin(0.1) & 0 \\ 0 & 1 \end{bmatrix} \begin{bmatrix} 1 \\ 0.1 \end{bmatrix}$$


   $$\mathbf{\hat{x}}_t^- = \begin{bmatrix} 2 \\ 3 \\ 0.1 \end{bmatrix} + \begin{bmatrix} \cos(0.1) \\ \sin(0.1) \\ 0.1 \end{bmatrix} \approx \begin{bmatrix} 2.995 \\ 3.0998 \\ 0.2 \end{bmatrix}$$


   $$\mathbf{P}_t^- = \mathbf{A} \mathbf{P}_{t-1} \mathbf{A}^T + \mathbf{Q}_t = \mathbf{P}_{t-1} + \mathbf{Q}_t = \begin{bmatrix} 0.1 & 0 & 0 \\ 0 & 0.1 & 0 \\ 0 & 0 & 0.1 \end{bmatrix} + \begin{bmatrix} 0.01 & 0 & 0 \\ 0 & 0.01 & 0 \\ 0 & 0 & 0.01 \end{bmatrix} = \begin{bmatrix} 0.11 & 0 & 0 \\ 0 & 0.11 & 0 \\ 0 & 0 & 0.11 \end{bmatrix}$$


2. **Update Step**

   $$\mathbf{C} = \begin{bmatrix} 1 & 0 & 0 \\ 0 & 1 & 0 \end{bmatrix}$$

   $$\mathbf{y}_t = \mathbf{z}_t - \mathbf{C} \mathbf{\hat{x}}_t^- = \begin{bmatrix} 2.1 \\ 3.1 \end{bmatrix} - \begin{bmatrix} 1 & 0 & 0 \\ 0 & 1 & 0 \end{bmatrix} \begin{bmatrix} 2.995 \\ 3.0998 \\ 0.2 \end{bmatrix} = \begin{bmatrix} 2.1 \\ 3.1 \end{bmatrix} - \begin{bmatrix} 2.995 \\ 3.0998 \end{bmatrix} = \begin{bmatrix} -0.895 \\ 0.0002 \end{bmatrix}$$

   $$\mathbf{S}_t = \mathbf{C} \mathbf{P}_t^- \mathbf{C}^T + \mathbf{R}_t = \mathbf{C} \mathbf{P}_t^- \mathbf{C}^T + \mathbf{R}_t = \begin{bmatrix} 1 & 0 & 0 \\ 0 & 1 & 0 \end{bmatrix} \begin{bmatrix} 0.11 & 0 & 0 \\ 0 & 0.11 & 0 \\ 0 & 0 & 0.11 \end{bmatrix} \begin{bmatrix} 1 & 0 \\ 0 & 1 \\ 0 & 0 \end{bmatrix} + \begin{bmatrix} 0.05 & 0 \\ 0 & 0.05 \end{bmatrix} = \begin{bmatrix} 0.16 & 0 \\ 0 & 0.16 \end{bmatrix}$$


   $$\mathbf{K}_t = \mathbf{P}_t^- \mathbf{C}^T \mathbf{S}_t^{-1} = \begin{bmatrix} 0.11 & 0 & 0 \\ 0 & 0.11 & 0 \\ 0 & 0 & 0.11 \end{bmatrix} \begin{bmatrix} 1 & 0 \\ 0 & 1 \\ 0 & 0 \end{bmatrix} \begin{bmatrix} 0.16 & 0 \\ 0 & 0.16 \end{bmatrix}^{-1} = \begin{bmatrix} 0.11 & 0 \\ 0 & 0.11 \\ 0 & 0 \end{bmatrix} \begin{bmatrix} 6.25 & 0 \\ 0 & 6.25 \end{bmatrix} = \begin{bmatrix} 0.6875 & 0 \\ 0 & 0.6875 \\ 0 & 0 \end{bmatrix}$$


   $$\mathbf{\hat{x}}_t = \mathbf{\hat{x}}_t^- + \mathbf{K}_t \mathbf{y}_t = \begin{bmatrix} 2.995 \\ 3.0998 \\ 0.2 \end{bmatrix} + \begin{bmatrix} 0.6875 & 0 \\ 0 & 0.6875 \\ 0 & 0 \end{bmatrix} \begin{bmatrix} -0.895 \\ 0.0002 \end{bmatrix} = \begin{bmatrix} 2.995 \\ 3.0998 \\ 0.2 \end{bmatrix} + \begin{bmatrix} -0.615 \\ 0.0001375 \\ 0 \end{bmatrix} = \begin{bmatrix} 2.38 \\ 3.0999375 \\ 0.2 \end{bmatrix}$$



   $$\mathbf{P}_t = (\mathbf{I} - \mathbf{K}_t \mathbf{C}) \mathbf{P}_t^- = \left( \begin{bmatrix} 1 & 0 & 0 \\ 0 & 1 & 0 \\ 0 & 0 & 1 \end{bmatrix} - \begin{bmatrix} 0.6875 & 0 \\ 0 & 0

.6875 \\ 0 & 0 \end{bmatrix} \begin{bmatrix} 1 & 0 & 0 \\ 0 & 1 & 0 \end{bmatrix} \right) \begin{bmatrix} 0.11 & 0 & 0 \\ 0 & 0.11 & 0 \\ 0 & 0 & 0.11 \end{bmatrix}$$



   $$\mathbf{P}_t = \left( \begin{bmatrix} 1 & 0 & 0 \\ 0 & 1 & 0 \\ 0 & 0 & 1 \end{bmatrix} - \begin{bmatrix} 0.6875 & 0 & 0 \\ 0 & 0.6875 & 0 \\ 0 & 0 & 0 \end{bmatrix} \right) \begin{bmatrix} 0.11 & 0 & 0 \\ 0 & 0.11 & 0 \\ 0 & 0 & 0.11 \end{bmatrix} = \begin{bmatrix} 0.034375 & 0 & 0 \\ 0 & 0.034375 & 0 \\ 0 & 0 & 0.11 \end{bmatrix}$$


### Python Code Implementation

Here is the Python code to perform the above calculations:

```python
import numpy as np

# Initial state and covariance
x_hat_prev = np.array([2, 3, 0.1])
P_prev = np.array([[0.1, 0, 0],
                   [0, 0.1, 0],
                   [0, 0, 0.1]])

# Control input
u_t = np.array([1, 0.1])

# Process noise covariance
Q_t = np.array([[0.01, 0, 0],
                [0, 0.01, 0],
                [0, 0, 0.01]])

# Observation
z_t = np.array([2.1, 3.1])

# Observation noise covariance
R_t = np.array([[0.05, 0],
                [0, 0.05]])

# Motion model matrices
A = np.eye(3)
B = np.array([[np.cos(0.1), 0],
              [np.sin(0.1), 0],
              [0, 1]])

# Prediction step
x_hat_pred = A @ x_hat_prev + B @ u_t
P_pred = A @ P_prev @ A.T + Q_t

# Observation model matrix
C = np.array([[1, 0, 0],
              [0, 1, 0]])

# Innovation
y_t = z_t - C @ x_hat_pred

# Innovation covariance
S_t = C @ P_pred @ C.T + R_t

# Kalman gain
K_t = P_pred @ C.T @ np.linalg.inv(S_t)

# Update step
x_hat = x_hat_pred + K_t @ y_t
P_t = (np.eye(3) - K_t @ C) @ P_pred

print("Updated state estimate:\n", x_hat)
print("Updated covariance:\n", P_t)
```
